FY/Semantics.v
@@ -4,37 +4,41 @@ From Coq Require Import Arith.Arith.
 From Coq Require Import Arith.EqNat.
 From Coq Require Import Lists.List.
 From Coq Require Import Strings.String.
+From Coq Require Import Sets.Ensembles.
 From FY Require Export Utils.
 From FY Require Export Syntax.
 From FY Require Export State.
 Import ListNotations.
 
-Inductive ceval {nq}: com -> list ((total_map nat)*(Unitary nq)) -> list ((total_map nat)*(Unitary nq)) -> Prop :=
-  | E_Skip : forall st,
-      ceval <{ skip }> st st
-  | E_Ass : forall st a x,
-      ceval <{ x := a }> st (UpdateStateAssign nq st x a)
-  | E_Init : forall st,
-      ceval <{ new_qubit }> st (UpdateStateInit nq st)
-  | E_AppOne : forall st U m,
-      ceval <{ q m *= U }> st (UpdateStateApply nq st m U)
-  | E_AppTwo : forall st U m r,
-      ceval <{ q m r *= U }> st (UpdateStateApply nq st m U)
-  | E_Meas : forall st x m,
-      ceval <{ x :=meas m }> st (UpdateStateMeasure nq st x m)
-  | E_Seq : forall c1 c2 st st' st'',
-      ceval c1 st st' ->
-      ceval c2 st' st'' ->
-      ceval <{ c1 ; c2 }> st st''
-  | E_IfTrue : forall st st' b c1 c2,
-      ceval c1 (Filter nq st b) st' ->
-      ceval <{ if b then c1 else c2 end }> st st'
-  | E_IfFalse : forall st st' b c1 c2,
-      ceval c2 (FilterNeg nq st b) st' ->
-      ceval <{ if b then c1 else c2 end }> st st'
-  | E_WhileTrue : forall st st' st'' b c,
-      ceval c (Filter nq st b) st' ->
-      ceval <{ while b do c end }> (Filter nq st b) st' ->
-      ceval <{ while b do c end }> st' st''
-  | E_WhileFalse : forall st b c,
-      ceval <{ while b do c end }> (FilterNeg nq st b) (FilterNeg nq st b).
+Inductive ceval : nat -> nat -> com 
+    -> list ((total_map nat)*(Unitary 1%nat))
+    -> list ((total_map nat)*(Unitary 1%nat)) 
+    -> Prop :=
+  | E_Skip : forall n st,
+      ceval n n <{ skip }> st st
+  | E_Ass : forall n st a x,
+      ceval n n <{ x := a }> st (UpdateStateAssign n st x a)
+  | E_Init : forall n st,
+      ceval n (n + 1%nat) <{ new_qubit }> st (UpdateStateInit n st)
+  | E_AppOne : forall n st U m,
+      ceval n n <{ q m *= U }> st (UpdateStateApply n st m U)
+  | E_AppTwo : forall n st U m r,
+      ceval n n <{ q m r *= U }> st (UpdateStateApply n st m U)
+  | E_Meas : forall n st x m,
+      ceval n n <{ x :=meas m }> st (UpdateStateMeasure n st x m)
+  | E_Seq : forall n n' n'' c1 c2 st st' st'',
+      ceval n n' c1 st st' ->
+      ceval n' n'' c2 st' st'' ->
+      ceval n n'' <{ c1 ; c2 }> st st''
+  | E_IfTrue : forall n n' st st' b c1 c2,
+      ceval n n' c1 (Filter n st b) st' ->
+      ceval n n' <{ if b then c1 else c2 end }> st st'
+  | E_IfFalse : forall n n' st st' b c1 c2,
+      ceval  n n' c2 (FilterNeg n st b) st' ->
+      ceval n n' <{ if b then c1 else c2 end }> st st'
+  | E_WhileTrue : forall n n' st st' st'' b c,
+      ceval n n' c (Filter n st b) st' ->
+      ceval n n' <{ while b do c end }> (Filter n st b) st' ->
+      ceval n n' <{ while b do c end }> st' st''
+  | E_WhileFalse : forall n n' st b c,
+      ceval n n' <{ while b do c end }> (FilterNeg n st b) (FilterNeg n st b).
