FY/Logic.v
@@ -7,7 +7,7 @@ From FY Require Export Assertion.
 
 Definition hoare_triple 
     (np nq: nat)(P : Assertion np) (c : com) (Q : Assertion nq) : Prop :=
-    forall ns1 ns2 st1 st2, ceval c st1 st2 -> Cnorm (Expectation ns1 np st1 P) <= Cnorm (Expectation ns2 nq st2 Q).
+    forall ns1 ns2 st1 st2, ceval np np c st1 st2 -> Cnorm (Expectation ns1 np st1 P) <= Cnorm (Expectation ns2 nq st2 Q).
 
 Theorem equal_expectations: forall ns1 ns2 np nq P st, 
   Cnorm (Expectation ns1 np st P) <= Cnorm (Expectation ns2 nq st P).
